Cslib/Computability/LambdaCalculus/LocallyNameless/Context.lean
@@ -17,7 +17,7 @@ Contexts as pairs of free variables and types.
 
 universe u v
 
-variable {Var : Type u} {Ty : Type v} [DecidableEq Var]
+variable {Var : Type u} {Ty : Type v} [DecidableEq Var] [Inhabited Ty]
 
 namespace LambdaCalculus.LocallyNameless
 
@@ -40,32 +40,67 @@ instance : HasWellFormed (Context Var Ty) :=
 
 variable {Γ Δ : Context Var Ty}
 
+omit [DecidableEq Var] [Inhabited Ty] in
+@[grind _=_]
+theorem haswellformed_def : Γ✓ = Γ.NodupKeys := by rfl
+
+omit [Inhabited Ty] in
 /-- Context membership is preserved on permuting a context. -/
 theorem dom_perm_mem_iff (h : Γ.Perm Δ) {x : Var} : x ∈ Γ.dom ↔ x ∈ Δ.dom := by
   induction h <;> simp_all only [dom, Function.comp_apply, mem_toFinset, keys_cons, mem_cons] 
   grind
 
+instance : GetElem? (Context Var Ty) Var Ty (fun Γ x => x ∈ Γ.dom) where
+  getElem Γ x _ := List.dlookup x Γ |>.get!
+  getElem? Γ x := List.dlookup x Γ
+
+@[grind _=_]
+theorem getElem?_def : Γ[x]? = List.dlookup x Γ := by rfl
+
+omit [Inhabited Ty] in
 /-- Context membership implies membership in the domain. -/
 @[scoped grind →]
 theorem dom_mem (mem : ⟨x, σ⟩ ∈ Γ) : x ∈ Γ.dom := by
   simp only [dom, Function.comp_apply, mem_toFinset, keys]
   grind
 
--- TODO: shouldn't need to restate this, but some downstream grind doesn't work without it
--- TODO: instead of =, use ∈ notation on option? (may be why grind wasn't working)
 @[scoped grind →]
-theorem of_mem_dlookup (mem : Γ.dlookup x = some T) : ⟨x, T⟩ ∈ Γ := by
+theorem of_mem_dlookup (mem : T ∈ Γ[x]?) : ⟨x, T⟩ ∈ Γ := by
   exact List.of_mem_dlookup mem
 
-omit [DecidableEq Var] in
+omit [DecidableEq Var] [Inhabited Ty] in
 /-- Context well-formedness is preserved on permuting a context. -/
 @[scoped grind →]
 theorem wf_perm (h : Γ.Perm Δ) : Γ✓ → Δ✓ := (List.perm_nodupKeys h).mp
 
-omit [DecidableEq Var] in
+omit [DecidableEq Var] [Inhabited Ty] in
 /-- Context well-formedness is preserved on removing an element. -/
 @[scoped grind →]
 theorem wf_strengthen (ok : (Δ ++ ⟨x, σ⟩ :: Γ)✓) : (Δ ++ Γ)✓ := by
   exact List.NodupKeys.sublist (by simp) ok
 
 end LambdaCalculus.LocallyNameless.Context
+
+namespace List
+
+variable {α : Type u} {β : α → Type v} [DecidableEq α]
+
+-- TODO: this should upstream to Mathlib
+theorem sublist_dlookup (l₁ l₂ : List (Sigma β)) (nd₁ : l₁.NodupKeys) (nd₂ : l₂.NodupKeys)
+    (s : l₁ <+ l₂) (mem : b ∈ l₁.dlookup a) : l₂.dlookup a = some b := by
+  induction s generalizing a b
+  case slnil => exact mem
+  case cons p' _ ih =>
+    obtain ⟨a', b'⟩ := p'
+    have : a ≠ a' := by
+      have := ih nd₁ ?_ mem |> of_mem_dlookup |> mem_keys_of_mem
+      all_goals grind [nodupKeys_cons]
+    simp_all
+  case cons₂ p' _ ih =>
+    obtain ⟨a', b'⟩ := p'
+    by_cases h : a = a'
+    · subst h
+      rw [List.dlookup_cons_eq] at *
+      exact mem
+    · simp_all
+end List
